Finish porting what was finished of ADTs to Comp
Everything up to and including the example of refinement using ADTs now uses
Comp.  I'm not exactly sure what comes next, but I have a bit of an idea about
what to explore.  I think what comes next is cleaning up the example of
refinement, and then working on porting the examples in Computation.v to use
ADTs, and then find some more algorithms to play with.

ComputationalADT.v
@@ -4,350 +4,354 @@ Require Import Common Computation.
 Generalizable All Variables.
 Set Implicit Arguments.
 
-(** * Basic ADT definitions *)
-
-(** Hoare logic-style total correctness specification of a mutator method *)
-Definition mutatorMethodSpec (Ty : Type) :=
-  Ty    (* Initial model *)
-  -> nat (* Actual argument*)
-  -> Ty (* Final model *)
-  (*  -> nat (* Return value *) *)
-  -> Prop.
-
-(** Hoare logic-style total correctness specification of an obeserver method *)
-Definition observerMethodSpec (Ty : Type) :=
-  Ty    (* Initial model *)
-  -> nat (* Actual argument*)
-  (*  -> Ty (* Final model *) *)
-  -> nat (* Return value *)
-  -> Prop.
-
-(** Interface of an ADT *)
-Record ADT :=
-  {
-    Model : Type;
-    (** The way we model state mathematically *)
-
-    MutatorIndex : Type;
-    (** The index set of mutators *)
-
-    ObserverIndex : Type;
-    (** The index set of observers *)
-
-    MutatorMethodSpecs : MutatorIndex -> mutatorMethodSpec Model;
-    (** A specification for each mutator method *)
-
-    ObserverMethodSpecs : ObserverIndex -> observerMethodSpec Model
-  (** A specification for each observer method *)
-  }.
-
-(** Implementation type of a method *)
-Definition methodTypeD (State : Type) funcs :=
-  State -> nat -> Comp funcs (State * nat).
-
-(** Usual Hoare logic notion of implementating a mutator method spec *)
-
-Definition mutatorMethodCorrect (Model State : Type) funcs denote_funcs
-           (ms : mutatorMethodSpec Model)
-           (RepInv : Model -> State -> Prop)
-           (mb : methodTypeD State funcs)
-  := forall m s,
-       RepInv m s
-       -> forall x,
-            let s'y := mb s x in
-            forall s'y_value,
-              computes_to denote_funcs s'y s'y_value
-              -> exists m', RepInv m' (fst s'y_value)
-                            /\ ms m x m'
-                            /\ (snd s'y_value) = 0.
-
-Definition observerMethodCorrect (Model State : Type) funcs denote_funcs
-           (ms : observerMethodSpec Model)
-           (RepInv : Model -> State -> Prop)
-           (mb : methodTypeD State funcs)
-  := forall m s,
-       RepInv m s
-       -> forall x,
-            let s'y := mb s x in
-            forall s'y_value,
-              computes_to denote_funcs s'y s'y_value
-              -> RepInv m (fst s'y_value)
-                 /\ ms m x (snd s'y_value).
-
-(** One implementation of an ADT *)
-Record ADTimpl (A : ADT) funcs denote_funcs :=
-  {
-    State : Type;
-    (** Real state type in Gallina *)
-
-    RepInv : Model A -> State -> Prop;
-    (** Relationship between abstract (specification) and concrete (implementation) states *)
-
-    MutatorMethodBodies : MutatorIndex A -> methodTypeD State funcs;
-    (** An implementation of each mutator method *)
-
-    ObserverMethodBodies : ObserverIndex A -> methodTypeD State funcs;
-    (** An implementation of each observer method *)
-
-    MutatorMethodsCorrect : forall idx, mutatorMethodCorrect
-                                          denote_funcs
-                                          (MutatorMethodSpecs A idx)
-                                          RepInv
-                                          (MutatorMethodBodies idx);
-    (** All mutator methods satisfy their specs. *)
-
-    ObserverMethodsCorrect : forall idx, observerMethodCorrect
-                                           denote_funcs
-                                           (ObserverMethodSpecs A idx)
-                                           RepInv
-                                           (ObserverMethodBodies idx)
-  (** All observer methods satisfy their specs. *)
-  }.
-
-Ltac get_mut_spec_of_impl Ai :=
-  let A := match type of Ai with ADTimpl ?A _ => constr:(A) end in
+Ltac get_mut_spec_of_generic_impl ADTimpl MutatorMethodSpecs Ai :=
+  let A := match type of Ai with ADTimpl ?A => constr:(A) end in
   let AMutSpec' := constr:(MutatorMethodSpecs A) in
   let AMutSpec := (eval simpl in AMutSpec') in
   match goal with
     | [ H : AMutSpec _ _ _ _ |- _ ] => constr:(H)
   end.
-Ltac impl_has_mut_spec Ai := idtac; get_mut_spec_of_impl Ai.
+Ltac generic_impl_has_mut_spec ADTimpl MutatorMethodSpecs Ai := idtac; get_mut_spec_of_generic_impl ADTimpl MutatorMethodSpecs Ai.
 
-Ltac impl_t' :=
-  repeat match goal with
-           | _ => eassumption
-           | _ => intro
-           | _ => progress simpl in *
-           | _ => progress split_and
-           | _ => progress inversion_computes_to
-           | _ => progress subst
-           | _ => split
-           | _ => progress destruct_sum_in_match
-           | [ Ai : ADTimpl _ _ |- _ ] => eapply (ObserverMethodsCorrect Ai)
-           | [ Ai : ADTimpl _ _ |- _ ]
-             => (not_tac (impl_has_mut_spec Ai));
-               edestruct (MutatorMethodsCorrect Ai); try eassumption; [];
-               instantiate
-           | _ => progress apply_hyp
-         end.
+Ltac generic_impl_t'' ADTimpl MutatorMethodSpecs ObserverMethodsCorrect MutatorMethodsCorrect :=
+  match goal with
+    | _ => eassumption
+    | _ => intro
+    | _ => progress simpl in *
+    | _ => progress split_and
+    | _ => progress inversion_computes_to
+    | _ => progress subst
+    | _ => split
+    | _ => progress destruct_sum_in_match
+    | [ Ai : ADTimpl ?A |- _ ] => eapply (@ObserverMethodsCorrect A Ai)
+    | [ Ai : ADTimpl ?A |- _ ]
+      => (not_tac (generic_impl_has_mut_spec ADTimpl MutatorMethodSpecs Ai));
+        edestruct (@MutatorMethodsCorrect A Ai); try eassumption; [];
+        instantiate
+    | _ => progress apply_hyp
+  end.
 
-Ltac impl_t := repeat first [ progress impl_t'
-                            | eexists (_, _)
-                            | esplit ].
+Ltac generic_impl_t' ADTimpl MutatorMethodSpecs ObserverMethodsCorrect MutatorMethodsCorrect :=
+  repeat generic_impl_t'' ADTimpl MutatorMethodSpecs ObserverMethodsCorrect MutatorMethodsCorrect.
 
-(** * A simple pairing combinator *)
+Ltac generic_impl_t ADTimpl MutatorMethodSpecs ObserverMethodsCorrect MutatorMethodsCorrect :=
+  repeat first [ progress generic_impl_t' ADTimpl MutatorMethodSpecs ObserverMethodsCorrect MutatorMethodsCorrect
+               | eexists (_, _)
+               | esplit
+               | progress eapply_hyp' ].
 
-Section paired.
-  Variables A B : ADT.
-  (** Let's compose these two ADTs. *)
-
-  Variable mutatorIndex : Type.
-  Variable observerIndex : Type.
-  Variable mutatorMap : mutatorIndex -> MutatorIndex A * MutatorIndex B.
-  Variable observerMap : observerIndex -> ObserverIndex A + ObserverIndex B.
-
-  (** The composed ADT *)
-  Definition pairedADT :=
-    {|
-      Model := Model A * Model B;
-      MutatorIndex := mutatorIndex;
-      ObserverIndex := observerIndex;
-      MutatorMethodSpecs idx :=
-        let s := mutatorMap idx in
-        fun m x m' => MutatorMethodSpecs A (fst s) (fst m) x (fst m')
-                      /\ MutatorMethodSpecs B (snd s) (snd m) x (snd m');
-      ObserverMethodSpecs idx :=
-        fun m x y => match observerMap idx with
-                       | inl idx' => ObserverMethodSpecs A idx' (fst m) x y
-                       | inr idx' => ObserverMethodSpecs B idx' (snd m) x y
-                     end
-    |}.
-
-  (** Now we show how to implement it. *)
+(** * Basic ADT definitions *)
+Section comp_env.
+  (** We have one ambiant [funcs] and [denote_funcs] around for everything. *)
   Variable funcs : string -> Type * Type.
   Variable denote_funcs : forall name, fst (funcs name) -> Comp funcs (snd (funcs name)).
-  Variable Ai : ADTimpl A denote_funcs.
-  Variable Bi : ADTimpl B denote_funcs.
 
-  Definition pairedImpl : ADTimpl pairedADT denote_funcs.
-  Proof.
-    refine {|
-        State := State Ai * State Bi;
-        RepInv := fun (m : Model pairedADT) s
-                  => RepInv Ai (fst m) (fst s)
-                     /\ RepInv Bi (snd m) (snd s);
-        MutatorMethodBodies name :=
-          fun s x
-          => (x'1 <- MutatorMethodBodies Ai (fst (mutatorMap name)) (fst s) x;
-              x'2 <- MutatorMethodBodies Bi (snd (mutatorMap name)) (snd s) x;
-              ret ((fst x'1, fst x'2), 0))%comp;
-        ObserverMethodBodies name :=
-          fun s x
-          => match observerMap name with
-               | inl name'
-                 => let sy := ObserverMethodBodies Ai name' (fst s) x in
-                    (sy' <- sy;
-                     ret ((fst sy', snd s), snd sy'))%comp
-               | inr name'
-                 => let sy := ObserverMethodBodies Bi name' (snd s) x in
-                    (sy' <- sy;
-                     ret ((fst s, fst sy'), snd sy'))%comp
-             end
-      |};
-    abstract impl_t.
-  Defined.
-End paired.
+  (** Hoare logic-style total correctness specification of a mutator method *)
+  Definition mutatorMethodSpec (Ty : Type) :=
+    Ty    (* Initial model *)
+    -> nat (* Actual argument*)
+    -> Ty (* Final model *)
+    (*  -> nat (* Return value *) *)
+    -> Prop.
 
-Section prod.
-  Variable model : Type.
-  Variables AMutIndex BMutIndex AObsIndex BObsIndex : Type.
-  Variable AMutSpec : AMutIndex -> mutatorMethodSpec model.
-  Variable BMutSpec : BMutIndex -> mutatorMethodSpec model.
-  Variable AObsSpec : AObsIndex -> observerMethodSpec model.
-  Variable BObsSpec : BObsIndex -> observerMethodSpec model.
+  (** Hoare logic-style total correctness specification of an obeserver method *)
+  Definition observerMethodSpec (Ty : Type) :=
+    Ty    (* Initial model *)
+    -> nat (* Actual argument*)
+    (*  -> Ty (* Final model *) *)
+    -> nat (* Return value *)
+    -> Prop.
 
-  Let A := {| Model := model;
-              MutatorMethodSpecs := AMutSpec;
-              ObserverMethodSpecs := AObsSpec |}.
-  Let B := {| Model := model;
-              MutatorMethodSpecs := BMutSpec;
-              ObserverMethodSpecs := BObsSpec |}.
+  (** Interface of an ADT *)
+  Record ADT :=
+    {
+      Model : Type;
+      (** The way we model state mathematically *)
 
-  Variable mutatorIndex : Type.
-  Variable observerIndex : Type.
-  Variable mutatorMap : mutatorIndex -> MutatorIndex A * MutatorIndex B.
-  Variable observerMap : observerIndex -> ObserverIndex A + ObserverIndex B.
+      MutatorIndex : Type;
+      (** The index set of mutators *)
 
-  (** Let's compose these two ADTs. *)
-  (** The composed ADT, which doesn't duplicate models *)
-  Definition prodADT :=
-    {|
-      Model := model;
-      MutatorMethodSpecs idx :=
-        fun m x m' => MutatorMethodSpecs A (fst (mutatorMap idx)) m x m'
-                      /\ MutatorMethodSpecs B (snd (mutatorMap idx)) m x m';
-      ObserverMethodSpecs idx :=
-        fun m x y => match observerMap idx with
-                       | inl idx' => ObserverMethodSpecs A idx' m x y
-                       | inr idx' => ObserverMethodSpecs B idx' m x y
-                     end
-    |}.
+      ObserverIndex : Type;
+      (** The index set of observers *)
 
-  (** Now we show how to implement it. *)
-  Variable funcs : string -> Type * Type.
-  Variable denote_funcs : forall name, fst (funcs name)
-                                       -> Comp funcs (snd (funcs name)).
-  Variable Ai : ADTimpl A denote_funcs.
-  Variable Bi : ADTimpl B denote_funcs.
+      MutatorMethodSpecs : MutatorIndex -> mutatorMethodSpec Model;
+      (** A specification for each mutator method *)
 
-  (*Local Hint Extern 1 (@ex (_ * _) _) => eexists (_, _).*)
+      ObserverMethodSpecs : ObserverIndex -> observerMethodSpec Model
+    (** A specification for each observer method *)
+    }.
 
-  Hypothesis mutators_match
-  : forall idx,
-    forall m x m' m'',
-      AMutSpec (fst (mutatorMap idx)) m x m'
-      -> BMutSpec (snd (mutatorMap idx)) m x m''
-      -> m' = m''.
+  (** Implementation type of a method *)
+  Definition methodTypeD (State : Type) :=
+    State -> nat -> Comp funcs (State * nat).
 
-  Local Hint Extern 1 => apply symmetry.
+  (** Usual Hoare logic notion of implementating a mutator method spec *)
 
-  Definition prodImpl : ADTimpl prodADT denote_funcs.
-    refine {|
-        State := State Ai * State Bi;
-        RepInv := fun (m : Model prodADT) s
-                  => RepInv Ai m (fst s)
-                     /\ RepInv Bi m (snd s);
-        MutatorMethodBodies idx :=
-          fun s x =>
-            (s1 <- MutatorMethodBodies Ai (fst (mutatorMap idx)) (fst s) x;
-             s2 <- MutatorMethodBodies Bi (snd (mutatorMap idx)) (snd s) x;
-             ret ((fst s1, fst s2), 0))%comp;
-        ObserverMethodBodies idx :=
-          match observerMap idx with
-            | inl idx' =>
-              fun s x =>
-                (s'y <- ObserverMethodBodies Ai idx' (fst s) x;
-                 ret ((fst s'y, snd s), snd s'y))%comp
-            | inr idx' =>
-              fun s x =>
-                (s'y <- ObserverMethodBodies Bi idx' (snd s) x;
-                 ret ((fst s, fst s'y), snd s'y))%comp
-          end
-      |};
-    abstract (
-        intro idx;
-        try (assert (MM := mutators_match idx));
-        impl_t';
-        match goal with
-          | [ AM : AMutSpec _ _ _ _, BM : BMutSpec _ _ _ _ |- _ ]
-            => specialize (MM _ _ _ _ AM BM); subst
-        end;
-        impl_t
-      ).
-  Defined.
-End prod.
+  Definition mutatorMethodCorrect (Model State : Type)
+             (ms : mutatorMethodSpec Model)
+             (RepInv : Model -> State -> Prop)
+             (mb : methodTypeD State)
+    := forall m s,
+         RepInv m s
+         -> forall x,
+              let s'y := mb s x in
+              forall s'y_value,
+                computes_to denote_funcs s'y s'y_value
+                -> exists m', RepInv m' (fst s'y_value)
+                              /\ ms m x m'
+                              /\ (snd s'y_value) = 0.
 
-(** A transformation (approximately, injection) from one ADT to another *)
+  Definition observerMethodCorrect (Model State : Type)
+             (ms : observerMethodSpec Model)
+             (RepInv : Model -> State -> Prop)
+             (mb : methodTypeD State)
+    := forall m s,
+         RepInv m s
+         -> forall x,
+              let s'y := mb s x in
+              forall s'y_value,
+                computes_to denote_funcs s'y s'y_value
+                -> RepInv m (fst s'y_value)
+                   /\ ms m x (snd s'y_value).
 
-Section inj.
-  Variables A B : ADT.
-  (** Let's compose these two ADTs. *)
+  (** One implementation of an ADT *)
+  Record ADTimpl (A : ADT) :=
+    {
+      State : Type;
+      (** Real state type in Gallina *)
 
-  Variable BtoA : Model B -> Model A.
-  Variable mutatorMap : MutatorIndex B -> MutatorIndex A.
-  Variable observerMap : ObserverIndex B -> ObserverIndex A.
-  Hypothesis mutatorSpecMap
-  : forall idx m x m',
-      MutatorMethodSpecs A (mutatorMap idx) (BtoA m) x m'
-      -> exists m'',
-           m' = BtoA m''
-           /\ MutatorMethodSpecs B idx m x m''.
-  Hypothesis observerSpecMap
-  : forall idx m x y,
-      ObserverMethodSpecs A (observerMap idx) (BtoA m) x y
-      -> ObserverMethodSpecs B idx m x y.
+      RepInv : Model A -> State -> Prop;
+      (** Relationship between abstract (specification) and concrete (implementation) states *)
 
-  Variable funcs : string -> Type * Type.
-  Variable denote_funcs : forall name, fst (funcs name) -> Comp funcs (snd (funcs name)).
-  Variable Ai : ADTimpl A denote_funcs.
+      MutatorMethodBodies : MutatorIndex A -> methodTypeD State;
+      (** An implementation of each mutator method *)
 
-  Definition injImpl : ADTimpl B denote_funcs.
-  Proof.
-    refine {|
-        State := State Ai;
-        RepInv := fun (m : Model B) s
-                  => RepInv Ai (BtoA m) s;
-        MutatorMethodBodies name := MutatorMethodBodies Ai (mutatorMap name);
-        ObserverMethodBodies name := ObserverMethodBodies Ai (observerMap name)
-      |};
-    abstract (
-        impl_t';
-        edestruct mutatorSpecMap; try eassumption;
-        impl_t
-      ).
-  Defined.
-End inj.
+      ObserverMethodBodies : ObserverIndex A -> methodTypeD State;
+      (** An implementation of each observer method *)
+
+      MutatorMethodsCorrect : forall idx, mutatorMethodCorrect
+                                            (MutatorMethodSpecs A idx)
+                                            RepInv
+                                            (MutatorMethodBodies idx);
+      (** All mutator methods satisfy their specs. *)
+
+      ObserverMethodsCorrect : forall idx, observerMethodCorrect
+                                             (ObserverMethodSpecs A idx)
+                                             RepInv
+                                             (ObserverMethodBodies idx)
+    (** All observer methods satisfy their specs. *)
+    }.
+
+  Ltac impl_t'' := generic_impl_t'' ADTimpl MutatorMethodSpecs ObserverMethodsCorrect MutatorMethodsCorrect.
+  Ltac impl_t' := generic_impl_t' ADTimpl MutatorMethodSpecs ObserverMethodsCorrect MutatorMethodsCorrect.
+  Ltac impl_t := generic_impl_t ADTimpl MutatorMethodSpecs ObserverMethodsCorrect MutatorMethodsCorrect.
+
+  (** * A simple pairing combinator *)
+
+  Section paired.
+    Variables A B : ADT.
+    (** Let's compose these two ADTs. *)
+
+    Variable mutatorIndex : Type.
+    Variable observerIndex : Type.
+    Variable mutatorMap : mutatorIndex -> MutatorIndex A * MutatorIndex B.
+    Variable observerMap : observerIndex -> ObserverIndex A + ObserverIndex B.
+
+    (** The composed ADT *)
+    Definition pairedADT :=
+      {|
+        Model := Model A * Model B;
+        MutatorIndex := mutatorIndex;
+        ObserverIndex := observerIndex;
+        MutatorMethodSpecs idx :=
+          let s := mutatorMap idx in
+          fun m x m' => MutatorMethodSpecs A (fst s) (fst m) x (fst m')
+                        /\ MutatorMethodSpecs B (snd s) (snd m) x (snd m');
+        ObserverMethodSpecs idx :=
+          fun m x y => match observerMap idx with
+                         | inl idx' => ObserverMethodSpecs A idx' (fst m) x y
+                         | inr idx' => ObserverMethodSpecs B idx' (snd m) x y
+                       end
+      |}.
+
+    (** Now we show how to implement it. *)
+    Variable Ai : ADTimpl A.
+    Variable Bi : ADTimpl B.
+
+    Definition pairedImpl : ADTimpl pairedADT.
+    Proof.
+      refine {|
+          State := State Ai * State Bi;
+          RepInv := fun (m : Model pairedADT) s
+                    => RepInv Ai (fst m) (fst s)
+                       /\ RepInv Bi (snd m) (snd s);
+          MutatorMethodBodies name :=
+            fun s x
+            => (x'1 <- MutatorMethodBodies Ai (fst (mutatorMap name)) (fst s) x;
+                x'2 <- MutatorMethodBodies Bi (snd (mutatorMap name)) (snd s) x;
+                ret ((fst x'1, fst x'2), 0))%comp;
+          ObserverMethodBodies name :=
+            fun s x
+            => match observerMap name with
+                 | inl name'
+                   => let sy := ObserverMethodBodies Ai name' (fst s) x in
+                      (sy' <- sy;
+                       ret ((fst sy', snd s), snd sy'))%comp
+                 | inr name'
+                   => let sy := ObserverMethodBodies Bi name' (snd s) x in
+                      (sy' <- sy;
+                       ret ((fst s, fst sy'), snd sy'))%comp
+               end
+        |};
+      abstract impl_t.
+    Defined.
+  End paired.
+
+  Section prod.
+    Variable model : Type.
+    Variables AMutIndex BMutIndex AObsIndex BObsIndex : Type.
+    Variable AMutSpec : AMutIndex -> mutatorMethodSpec model.
+    Variable BMutSpec : BMutIndex -> mutatorMethodSpec model.
+    Variable AObsSpec : AObsIndex -> observerMethodSpec model.
+    Variable BObsSpec : BObsIndex -> observerMethodSpec model.
+
+    Let A := {| Model := model;
+                MutatorMethodSpecs := AMutSpec;
+                ObserverMethodSpecs := AObsSpec |}.
+    Let B := {| Model := model;
+                MutatorMethodSpecs := BMutSpec;
+                ObserverMethodSpecs := BObsSpec |}.
+
+    Variable mutatorIndex : Type.
+    Variable observerIndex : Type.
+    Variable mutatorMap : mutatorIndex -> MutatorIndex A * MutatorIndex B.
+    Variable observerMap : observerIndex -> ObserverIndex A + ObserverIndex B.
+
+    (** Let's compose these two ADTs. *)
+    (** The composed ADT, which doesn't duplicate models *)
+    Definition prodADT :=
+      {|
+        Model := model;
+        MutatorMethodSpecs idx :=
+          fun m x m' => MutatorMethodSpecs A (fst (mutatorMap idx)) m x m'
+                        /\ MutatorMethodSpecs B (snd (mutatorMap idx)) m x m';
+        ObserverMethodSpecs idx :=
+          fun m x y => match observerMap idx with
+                         | inl idx' => ObserverMethodSpecs A idx' m x y
+                         | inr idx' => ObserverMethodSpecs B idx' m x y
+                       end
+      |}.
+
+    (** Now we show how to implement it. *)
+    Variable Ai : ADTimpl A.
+    Variable Bi : ADTimpl B.
+
+    (*Local Hint Extern 1 (@ex (_ * _) _) => eexists (_, _).*)
+
+    Hypothesis mutators_match
+    : forall idx,
+      forall m x m' m'',
+        AMutSpec (fst (mutatorMap idx)) m x m'
+        -> BMutSpec (snd (mutatorMap idx)) m x m''
+        -> m' = m''.
+
+    Local Hint Extern 1 => apply symmetry.
+
+    Definition prodImpl : ADTimpl prodADT.
+      refine {|
+          State := State Ai * State Bi;
+          RepInv := fun (m : Model prodADT) s
+                    => RepInv Ai m (fst s)
+                       /\ RepInv Bi m (snd s);
+          MutatorMethodBodies idx :=
+            fun s x =>
+              (s1 <- MutatorMethodBodies Ai (fst (mutatorMap idx)) (fst s) x;
+               s2 <- MutatorMethodBodies Bi (snd (mutatorMap idx)) (snd s) x;
+               ret ((fst s1, fst s2), 0))%comp;
+          ObserverMethodBodies idx :=
+            match observerMap idx with
+              | inl idx' =>
+                fun s x =>
+                  (s'y <- ObserverMethodBodies Ai idx' (fst s) x;
+                   ret ((fst s'y, snd s), snd s'y))%comp
+              | inr idx' =>
+                fun s x =>
+                  (s'y <- ObserverMethodBodies Bi idx' (snd s) x;
+                   ret ((fst s, fst s'y), snd s'y))%comp
+            end
+        |};
+      abstract (
+          intro idx;
+          try (assert (MM := mutators_match idx));
+          impl_t';
+          match goal with
+            | [ AM : AMutSpec _ _ _ _, BM : BMutSpec _ _ _ _ |- _ ]
+              => specialize (MM _ _ _ _ AM BM); subst
+          end;
+          impl_t
+        ).
+    Defined.
+  End prod.
+
+  (** A transformation (approximately, injection) from one ADT to another *)
+
+  Section inj.
+    Variables A B : ADT.
+    (** Let's compose these two ADTs. *)
+
+    Variable BtoA : Model B -> Model A.
+    Variable mutatorMap : MutatorIndex B -> MutatorIndex A.
+    Variable observerMap : ObserverIndex B -> ObserverIndex A.
+    Hypothesis mutatorSpecMap
+    : forall idx m x m',
+        MutatorMethodSpecs A (mutatorMap idx) (BtoA m) x m'
+        -> exists m'',
+             m' = BtoA m''
+             /\ MutatorMethodSpecs B idx m x m''.
+    Hypothesis observerSpecMap
+    : forall idx m x y,
+        ObserverMethodSpecs A (observerMap idx) (BtoA m) x y
+        -> ObserverMethodSpecs B idx m x y.
+
+    Variable Ai : ADTimpl A.
+
+    Definition injImpl : ADTimpl B.
+    Proof.
+      refine {|
+          State := State Ai;
+          RepInv := fun (m : Model B) s
+                    => RepInv Ai (BtoA m) s;
+          MutatorMethodBodies name := MutatorMethodBodies Ai (mutatorMap name);
+          ObserverMethodBodies name := ObserverMethodBodies Ai (observerMap name)
+        |};
+      abstract (
+          impl_t';
+          edestruct mutatorSpecMap; try eassumption;
+          impl_t
+        ).
+    Defined.
+  End inj.
 
 
-(** * An example, composing binary commutative associative calculators for computable nat multisets *)
+  (** * An example, composing binary commutative associative calculators for computable nat multisets *)
 
-Definition multiset := nat -> nat.
-Definition add (s : multiset) (n : nat) : multiset
-  := fun m => if eq_nat_dec n m
-              then S (s m)
-              else s m.
+  Definition multiset := nat -> nat.
+  Definition add (s : multiset) (n : nat) : multiset
+    := fun m => if eq_nat_dec n m
+                then S (s m)
+                else s m.
 
-Require Import Min Max List.
+  Require Import Min Max List.
 
-Coercion sumbooltobool A B : {A} + {B} -> bool := fun x => if x then true else false.
+  Coercion sumbooltobool A B : {A} + {B} -> bool := fun x => if x then true else false.
 
-Infix "<=" := le_dec : bool_scope.
-Infix "<" := lt_dec : bool_scope.
-Infix ">=" := ge_dec : bool_scope.
-Infix ">" := gt_dec : bool_scope.
-(*Infix "->" := implb : bool_scope.*)
+  Infix "<=" := le_dec : bool_scope.
+  Infix "<" := lt_dec : bool_scope.
+  Infix ">=" := ge_dec : bool_scope.
+  Infix ">" := gt_dec : bool_scope.
+  (*Infix "->" := implb : bool_scope.*)
 
-(*
+  (*
 Fixpoint make_specs model (spec_list : list (string * methodSpec model))
   := fun s
      => match spec_list with
@@ -376,979 +380,950 @@ Definition make_accessor
         /\ f n d n'.
 
 Arguments make_accessor / .
-     *)
+   *)
 
 
-Definition add_spec : mutatorMethodSpec multiset
-  := fun m x m' => forall k, m' k = (add m x) k.
+  Definition add_spec : mutatorMethodSpec multiset
+    := fun m x m' => forall k, m' k = (add m x) k.
 
-Arguments add_spec / .
+  Arguments add_spec / .
 
-Definition bin_op_spec (op : nat -> nat -> nat) (default_value : nat)
-: observerMethodSpec multiset
-  := fun m x n => exists l : list nat,
-                    (forall v, m v = count_occ eq_nat_dec l v)
-                    /\ match l with
-                         | nil => n = default_value
-                         | cons z zs => n = fold_right op z zs
-                       end.
+  Definition bin_op_spec (op : nat -> nat -> nat) (default_value : nat)
+  : observerMethodSpec multiset
+    := fun m x n => exists l : list nat,
+                      (forall v, m v = count_occ eq_nat_dec l v)
+                      /\ match l with
+                           | nil => n = default_value
+                           | cons z zs => n = fold_right op z zs
+                         end.
 
-Arguments bin_op_spec / .
+  Arguments bin_op_spec / .
 
-Definition NatBinOp
-           (op : nat -> nat -> nat)
-           (is_assoc : forall x y z, op x (op y z) = op (op x y) z)
-           (is_comm : forall x y, op x y = op y x)
-           (default_value : nat)
-: ADT
-  := {|
-      Model := multiset;
-      MutatorIndex := unit;
-      ObserverIndex := unit;
-      MutatorMethodSpecs u := add_spec;
-      ObserverMethodSpecs u := bin_op_spec op default_value
-    |}.
-
-Local Ltac rewrite_hyp' :=
-  match goal with
-    | [ H : _ |- _ ] => rewrite H
-  end.
-
-Local Obligation Tactic :=
-  eauto with arith;
-  try solve [ repeat match goal with
-                       | _ => progress (simpl; rewrite_hyp'; trivial)
-                       | [ |- _ -> _ ] => let x := fresh in intro x; induction x; trivial
-                     end
-            | intros; omega ].
-
-Program Definition NatLower default_value : ADT
-  := NatBinOp min _ _ default_value.
-
-Program Definition NatUpper default_value : ADT
-  := NatBinOp max _ _ default_value.
-
-Program Definition NatSum default_value : ADT
-  := NatBinOp plus _ _ default_value.
-
-Program Definition NatProd default_value : ADT
-  := NatBinOp mult _ _ default_value.
-
-
-Hint Immediate le_min_l le_min_r le_max_l le_max_r.
-
-Lemma min_trans : forall n m v,
-  n <= v
-  -> min n m <= v.
-  intros; destruct (min_spec n m); omega.
-Qed.
-
-Lemma max_trans : forall n m v,
-  n >= v
-  -> max n m >= v.
-  intros; destruct (max_spec n m); omega.
-Qed.
-
-Hint Resolve min_trans max_trans.
-
-Arguments add _ _ _ / .
-
-(*
-Section def_NatBinOpI.
-
-  Local Ltac induction_list_then tac :=
-    lazymatch goal with
-      | [ l : list _ |- _ ]
-        => repeat match goal with
-                    | [ H : appcontext[l] |- _ ] => clear H
-                  end;
-          induction l; tac
-    end.
-
-  Local Ltac manipulate_op op_assoc op_comm :=
-    match goal with
-      | _ => reflexivity
-      | _ => progress simpl in *
-      | _ => apply op_comm
-      | _ => rewrite <- ?op_assoc; revert op_assoc op_comm; rewrite_hyp'; intros
-      | _ => rewrite ?op_assoc; revert op_assoc op_comm; rewrite_hyp'; intros
-      | _ => rewrite <- ?op_assoc; f_equal; []
-      | _ => rewrite ?op_assoc; f_equal; []
-      | _ => apply op_comm
-    end.
-
-  Local Ltac deep_manipulate_op op op_assoc op_comm can_comm_tac :=
-    repeat match goal with
-             | _ => progress repeat manipulate_op op_assoc op_comm
-             | [ |- appcontext[op ?a ?b] ]
-               => can_comm_tac a b;
-                 rewrite (op_comm a b);
-                 let new_can_comm_tac :=
-                     fun x y =>
-                       can_comm_tac x y;
-                       try (unify x a;
-                            unify y b;
-                            fail 1 "Cannot commute" a "and" b "again")
-                 in deep_manipulate_op op op_assoc op_comm new_can_comm_tac
-           end.
-
-  Local Ltac solve_after_induction_list op op_assoc op_comm :=
-    solve [ deep_manipulate_op op op_assoc op_comm ltac:(fun a b => idtac) ].
-
-
-  Local Ltac t :=
-    repeat match goal with
-             | _ => assumption
-             | _ => intro
-             | _ => progress simpl in *
-             | [ |- appcontext[if string_dec ?A ?B then _ else _ ] ]
-               => destruct (string_dec A B)
-             | _ => progress subst
-             | [ H : ex _ |- _ ] => destruct H
-             | [ H : and _ _ |- _ ] => destruct H
-             | _ => split
-             | [ H : option _ |- _ ] => destruct H
-             | [ H : _ |- _ ] => solve [ inversion H ]
-             | [ |- appcontext[match ?x with _ => _ end] ] => destruct x
-             | [ H : appcontext[match ?x with _ => _ end] |- _  ] => destruct x
-             | [ H : Some _ = Some _ |- _ ] => inversion H; clear H
-             | _ => progress f_equal; []
-             | _ => progress intuition
-             | _ => repeat esplit; reflexivity
-             | [ H : _ |- _ ] => rewrite H; try (rewrite H; fail 1)
-           end.
-
-  Local Ltac t' op op_assoc op_comm :=
-    repeat first [ progress t
-                 | progress induction_list_then ltac:(solve_after_induction_list op op_assoc op_comm) ].
-
-  Definition NatBinOpI
-  : `(ADTimpl (@NatBinOp op op_assoc op_comm default_value)).
-  Proof.
-    intros.
-    refine {|
-        State := option nat;
-        RepInv := fun (m : Model (NatBinOp op op_assoc op_comm default_value)) n
-                  => exists l : list nat,
-                       (forall v, m v = count_occ eq_nat_dec l v)
-                       /\ match l with
-                            | nil => n = None
-                            | cons x xs => n = Some (fold_right op x xs)
-                          end;
-        MutatorMethodBodies u val x := (match val with
-                                          | None => Some x
-                                          | Some x' => Some (op x x')
-                                        end,
-                                        0);
-        ObserverMethodBodies u val x := (val,
-                                         match val with
-                                           | None => default_value
-                                           | Some x => x
-                                         end)
-      |};
-      intros [];
-      try solve [intros m [n|] [l [H0 H1]] x;
-                  (exists (add m x));
-                  repeat split;
-                  try (exists (x::l));
-                  abstract t' op op_assoc op_comm
-                | intros m [n|] [l [H0 H1]] x;
-                  repeat (split || exists m || exists l);
-                  abstract t' op op_assoc op_comm
-                | intros m [n|] [l [H0 H1]] x;
-                  [ repeat split;
-                    try (exists (add (fun _ => 0) n));
-                    repeat split;
-                    try (exists (n::nil));
-                    abstract (repeat split)
-                  | repeat split;
-                    try (exists m);
-                    repeat split;
-                    try (exists l);
-                    abstract (repeat split; assumption) ]
-                ].
-  Defined.
-End def_NatBinOpI.
-
-Definition NatLowerI default_val : ADTimpl (NatLower default_val)
-  := NatBinOpI _ _ _ _.
-
-Definition NatUpperI default_val : ADTimpl (NatUpper default_val)
-  := NatBinOpI _ _ _ _.
-
-Definition NatSumI default_val : ADTimpl (NatSum default_val)
-  := NatBinOpI _ _ _ _.
-
-Definition NatProdI default_val : ADTimpl (NatProd default_val)
-  := NatBinOpI _ _ _ _.
-
-Local Open Scope string_scope.
-
-Definition NatSumProd_spec : ADT
-  := {| Model := multiset;
+  Definition NatBinOp
+             (op : nat -> nat -> nat)
+             (is_assoc : forall x y z, op x (op y z) = op (op x y) z)
+             (is_comm : forall x y, op x y = op y x)
+             (default_value : nat)
+  : ADT
+    := {|
+        Model := multiset;
         MutatorIndex := unit;
-        ObserverIndex := unit + unit;
+        ObserverIndex := unit;
         MutatorMethodSpecs u := add_spec;
-        ObserverMethodSpecs u m x n :=
-          match u with
-            | inl _ => bin_op_spec plus 0 m x n
-            | inr _ => bin_op_spec mult 1 m x n
-          end
-     |}.
+        ObserverMethodSpecs u := bin_op_spec op default_value
+      |}.
 
-Record PartialADTimpl (A : ADT) :=
-  {
-    PState : Type;
-    (** Real state type in Gallina *)
+  Local Obligation Tactic :=
+    eauto with arith;
+    try solve [ repeat match goal with
+                         | _ => progress (simpl; rewrite_hyp'; trivial)
+                         | [ |- _ -> _ ] => let x := fresh in intro x; induction x; trivial
+                       end
+              | intros; omega ].
 
-    PRepInv : Model A -> PState -> Prop;
-    (** Relationship between abstract (specification) and concrete (implementation) states *)
+  Program Definition NatLower default_value : ADT
+    := NatBinOp min _ _ default_value.
 
-    PMutatorMethodBodies : MutatorIndex A -> methodTypeD PState;
-    (** An implementation of each mutator method *)
+  Program Definition NatUpper default_value : ADT
+    := NatBinOp max _ _ default_value.
 
-    PObserverMethodBodies : ObserverIndex A -> option (methodTypeD PState);
-    (** An implementation of each observer method *)
+  Program Definition NatSum default_value : ADT
+    := NatBinOp plus _ _ default_value.
 
-    PMutatorMethodsCorrect : forall idx, mutatorMethodCorrect
-                                           (MutatorMethodSpecs A idx)
-                                           PRepInv
-                                           (PMutatorMethodBodies idx);
-    (** All mutator methods satisfy their specs. *)
+  Program Definition NatProd default_value : ADT
+    := NatBinOp mult _ _ default_value.
 
-    PObserverMethodsCorrect : forall idx, match PObserverMethodBodies idx with
-                                            | Some body => observerMethodCorrect
-                                                             (ObserverMethodSpecs A idx)
-                                                             PRepInv
-                                                             body
+
+  Hint Immediate le_min_l le_min_r le_max_l le_max_r.
+
+  Lemma min_trans : forall n m v,
+                      n <= v
+                      -> min n m <= v.
+    intros; destruct (min_spec n m); omega.
+  Qed.
+
+  Lemma max_trans : forall n m v,
+                      n >= v
+                      -> max n m >= v.
+    intros; destruct (max_spec n m); omega.
+  Qed.
+
+  Hint Resolve min_trans max_trans.
+
+  Arguments add _ _ _ / .
+
+  Section def_NatBinOpI.
+
+    Local Ltac induction_list_then tac :=
+      lazymatch goal with
+  | [ l : list _ |- _ ]
+    => repeat match goal with
+                | [ H : appcontext[l] |- _ ] => clear H
+              end;
+      induction l; tac
+    end.
+
+    Local Ltac manipulate_op op_assoc op_comm :=
+      match goal with
+        | _ => reflexivity
+        | _ => progress simpl in *
+        | _ => apply op_comm
+        | _ => rewrite <- ?op_assoc; revert op_assoc op_comm; rewrite_hyp'; intros
+        | _ => rewrite ?op_assoc; revert op_assoc op_comm; rewrite_hyp'; intros
+        | _ => rewrite <- ?op_assoc; f_equal; []
+        | _ => rewrite ?op_assoc; f_equal; []
+        | _ => apply op_comm
+      end.
+
+    Local Ltac deep_manipulate_op op op_assoc op_comm can_comm_tac :=
+      repeat match goal with
+               | _ => progress repeat manipulate_op op_assoc op_comm
+               | [ |- appcontext[op ?a ?b] ]
+                 => can_comm_tac a b;
+                   rewrite (op_comm a b);
+                   let new_can_comm_tac :=
+                       fun x y =>
+                         can_comm_tac x y;
+                         try (unify x a;
+                              unify y b;
+                              fail 1 "Cannot commute" a "and" b "again")
+                   in deep_manipulate_op op op_assoc op_comm new_can_comm_tac
+             end.
+
+    Local Ltac solve_after_induction_list op op_assoc op_comm :=
+      solve [ deep_manipulate_op op op_assoc op_comm ltac:(fun a b => idtac) ].
+
+
+    Local Ltac t :=
+      repeat match goal with
+               | _ => assumption
+               | _ => intro
+               | _ => progress simpl in *
+               | [ |- appcontext[if string_dec ?A ?B then _ else _ ] ]
+                 => destruct (string_dec A B)
+               | _ => progress subst
+               | [ H : ex _ |- _ ] => destruct H
+               | [ H : and _ _ |- _ ] => destruct H
+               | _ => split
+               | [ H : option _ |- _ ] => destruct H
+               | [ H : _ |- _ ] => solve [ inversion H ]
+               | [ |- appcontext[match ?x with _ => _ end] ] => destruct x
+               | [ H : appcontext[match ?x with _ => _ end] |- _  ] => destruct x
+               | [ H : Some _ = Some _ |- _ ] => inversion H; clear H
+               | _ => progress f_equal; []
+               | _ => progress intuition
+               | _ => repeat esplit; reflexivity
+               | [ H : _ |- _ ] => rewrite H; try (rewrite H; fail 1)
+             end.
+
+    Local Ltac t' op op_assoc op_comm :=
+      repeat first [ progress t
+                   | progress induction_list_then ltac:(solve_after_induction_list op op_assoc op_comm) ].
+
+    Definition NatBinOpI
+    : `(ADTimpl (@NatBinOp op op_assoc op_comm default_value)).
+    Proof.
+      intros.
+      refine {|
+          State := option nat;
+          RepInv := fun (m : Model (NatBinOp op op_assoc op_comm default_value)) n
+                    => exists l : list nat,
+                         (forall v, m v = count_occ eq_nat_dec l v)
+                         /\ match l with
+                              | nil => n = None
+                              | cons x xs => n = Some (fold_right op x xs)
+                            end;
+          MutatorMethodBodies u val x := (ret (match val with
+                                                 | None => Some x
+                                                 | Some x' => Some (op x x')
+                                               end,
+                                               0))%comp;
+          ObserverMethodBodies u val x := (ret (val,
+                                                match val with
+                                                  | None => default_value
+                                                  | Some x => x
+                                                end))%comp
+        |};
+        intros [];
+        solve [ (intros m [n|] [l [H0 H1] ] x ? ?);
+                inversion_computes_to; subst; simpl in *;
+                (exists (add m x));
+                repeat split;
+                try (exists (x::l));
+                abstract t' op op_assoc op_comm
+              | intros m [n|] [l [H0 H1] ] x ? ?;
+                       inversion_computes_to; subst; simpl in *;
+                repeat (split || exists m || exists l);
+                abstract t' op op_assoc op_comm
+              | intros m [n|] [l [H0 H1] ] x ? ?;
+                       inversion_computes_to; subst; simpl in *;
+                [ repeat split;
+                  try (exists (add (fun _ => 0) n));
+                  repeat split;
+                  try (exists (n::nil));
+                  abstract (repeat split)
+                | repeat split;
+                  try (exists m);
+                  repeat split;
+                  try (exists l);
+                  abstract (repeat split; assumption) ]
+              ].
+    Defined.
+  End def_NatBinOpI.
+
+  Section nat_op_ex.
+    Variable default_val : nat.
+
+    Definition NatLowerI : ADTimpl (NatLower default_val)
+      := NatBinOpI _ _ _ _.
+
+    Definition NatUpperI : ADTimpl (NatUpper default_val)
+      := NatBinOpI _ _ _ _.
+
+    Definition NatSumI : ADTimpl (NatSum default_val)
+      := NatBinOpI _ _ _ _.
+
+    Definition NatProdI : ADTimpl (NatProd default_val)
+      := NatBinOpI _ _ _ _.
+  End nat_op_ex.
+
+  Local Open Scope string_scope.
+
+  Definition NatSumProd_spec : ADT
+    := {| Model := multiset;
+          MutatorIndex := unit;
+          ObserverIndex := unit + unit;
+          MutatorMethodSpecs u := add_spec;
+          ObserverMethodSpecs u m x n :=
+            match u with
+              | inl _ => bin_op_spec plus 0 m x n
+              | inr _ => bin_op_spec mult 1 m x n
+            end
+       |}.
+
+  Record PartialADTimpl (A : ADT) :=
+    {
+      PState : Type;
+      (** Real state type in Gallina *)
+
+      PRepInv : Model A -> PState -> Prop;
+      (** Relationship between abstract (specification) and concrete (implementation) states *)
+
+      PMutatorMethodBodies : MutatorIndex A -> methodTypeD PState;
+      (** An implementation of each mutator method *)
+
+      PObserverMethodBodies : ObserverIndex A -> option (methodTypeD PState);
+      (** An implementation of each observer method *)
+
+      PMutatorMethodsCorrect : forall idx, mutatorMethodCorrect
+                                             (MutatorMethodSpecs A idx)
+                                             PRepInv
+                                             (PMutatorMethodBodies idx);
+      (** All mutator methods satisfy their specs. *)
+
+      PObserverMethodsCorrect : forall idx, match PObserverMethodBodies idx with
+                                              | Some body => observerMethodCorrect
+                                                               (ObserverMethodSpecs A idx)
+                                                               PRepInv
+                                                               body
+                                              | None => True
+                                            end
+    (** All observer methods satisfy their specs. *)
+    }.
+
+  Definition IsFull_PartialADTimpl A (impl : PartialADTimpl A)
+    := forall idx, PObserverMethodBodies impl idx <> None.
+
+  Definition ADTimpl_of_PartialADTimpl A impl (H : @IsFull_PartialADTimpl A impl)
+  : ADTimpl A
+    := {|
+        State := PState impl;
+        RepInv := PRepInv impl;
+        MutatorMethodBodies := PMutatorMethodBodies impl;
+        ObserverMethodBodies := (fun idx : ObserverIndex A
+                                 => match PObserverMethodBodies impl idx
+                                          as b
+                                          return b <> None -> _
+                                    with
+                                      | Some body => fun _ => body
+                                      | None => fun x : None <> None
+                                                => match x eq_refl with end
+                                    end (H idx));
+        MutatorMethodsCorrect := PMutatorMethodsCorrect impl;
+        ObserverMethodsCorrect := (fun idx : ObserverIndex A =>
+                                     match
+                                       PObserverMethodBodies impl idx as b
+                                       return
+                                       (forall n : b <> None,
+                                          match b with
+                                            | Some body =>
+                                              observerMethodCorrect
+                                                (ObserverMethodSpecs A idx)
+                                                (PRepInv impl)
+                                                body
                                             | None => True
-                                          end
-  (** All observer methods satisfy their specs. *)
-  }.
+                                          end ->
+                                          observerMethodCorrect
+                                            (ObserverMethodSpecs A idx)
+                                            (PRepInv impl)
+                                            (match b with
+                                               | Some body => fun _ => body
+                                               | None => _
+                                             end n))
+                                     with
+                                       | Some m => fun _ corr => corr
+                                       | None => fun x : None <> None =>
+                                                   match x eq_refl with end
+                                     end
+                                       (H idx)
+                                       (PObserverMethodsCorrect impl idx))
+      |}.
 
-Definition IsFull_PartialADTimpl A (impl : PartialADTimpl A)
-  := forall idx, PObserverMethodBodies impl idx <> None.
-
-Definition ADTimpl_of_PartialADTimpl A impl (H : @IsFull_PartialADTimpl A impl)
-: ADTimpl A
-  := {|
-      State := PState impl;
-      RepInv := PRepInv impl;
-      MutatorMethodBodies := PMutatorMethodBodies impl;
-      ObserverMethodBodies := (fun idx : ObserverIndex A
-                               => match PObserverMethodBodies impl idx
-                                        as b
-                                        return b <> None -> _
-                                  with
-                                    | Some body => fun _ => body
-                                    | None => fun x : None <> None
-                                              => match x eq_refl with end
-                                  end (H idx));
-      MutatorMethodsCorrect := PMutatorMethodsCorrect impl;
-      ObserverMethodsCorrect := (fun idx : ObserverIndex A =>
-                                   match
-                                     PObserverMethodBodies impl idx as b
-                                     return
-                                     (forall n : b <> None,
-                                        match b with
-                                          | Some body =>
-                                            observerMethodCorrect
-                                              (ObserverMethodSpecs A idx)
-                                              (PRepInv impl)
-                                              body
-                                          | None => True
-                                        end ->
-                                        observerMethodCorrect
-                                          (ObserverMethodSpecs A idx)
-                                          (PRepInv impl)
-                                          (match b with
-                                             | Some body => fun _ => body
-                                             | None => _
-                                           end n))
-                                   with
-                                     | Some m => fun _ corr => corr
-                                     | None => fun x : None <> None =>
-                                                 match x eq_refl with end
-                                   end
-                                     (H idx)
-                                     (PObserverMethodsCorrect impl idx))
-    |}.
-
-Coercion PartialADTimpl_of_ADTimpl A (impl : ADTimpl A)
-: PartialADTimpl A
-  := {|
-      PState := State impl;
-      PRepInv := RepInv impl;
-      PMutatorMethodBodies := MutatorMethodBodies impl;
-      PObserverMethodBodies idx := Some (ObserverMethodBodies impl idx);
-      PMutatorMethodsCorrect := MutatorMethodsCorrect impl;
-      PObserverMethodsCorrect := ObserverMethodsCorrect impl
-    |}.
+  Coercion PartialADTimpl_of_ADTimpl A (impl : @ADTimpl A)
+  : PartialADTimpl A
+    := {|
+        PState := State impl;
+        PRepInv := RepInv impl;
+        PMutatorMethodBodies := MutatorMethodBodies impl;
+        PObserverMethodBodies idx := Some (ObserverMethodBodies impl idx);
+        PMutatorMethodsCorrect := MutatorMethodsCorrect impl;
+        PObserverMethodsCorrect := ObserverMethodsCorrect impl
+      |}.
 
 
-Section pairedPartial.
-  Variables A B : ADT.
-  (** Let's compose these two ADTs. *)
+  Ltac p_impl_t'' := generic_impl_t'' PartialADTimpl MutatorMethodSpecs PObserverMethodsCorrect PMutatorMethodsCorrect.
+  Ltac p_impl_t' := generic_impl_t' PartialADTimpl MutatorMethodSpecs PObserverMethodsCorrect PMutatorMethodsCorrect.
+  Ltac p_impl_t := generic_impl_t PartialADTimpl MutatorMethodSpecs PObserverMethodsCorrect PMutatorMethodsCorrect.
 
-  Variable mutatorIndex : Type.
-  Variable observerIndex : Type.
-  Variable mutatorMap : mutatorIndex -> MutatorIndex A * MutatorIndex B.
-  Variable observerMap : observerIndex -> ObserverIndex A + ObserverIndex B.
 
-  (** Now we show how to implement it. *)
-  Variable Ai : PartialADTimpl A.
-  Variable Bi : PartialADTimpl B.
+  Section pairedPartial.
+    Variables A B : ADT.
+    (** Let's compose these two ADTs. *)
 
-  Definition pairedPartialImpl
-  : PartialADTimpl (pairedADT A B mutatorMap observerMap).
-  Proof.
-    refine {|
-        PState := PState Ai * PState Bi;
-        PRepInv := fun (m : Model (pairedADT A B mutatorMap observerMap)) s
-                   => PRepInv Ai (fst m) (fst s)
-                      /\ PRepInv Bi (snd m) (snd s);
-        PMutatorMethodBodies name :=
-          fun s x
-          => ((fst (PMutatorMethodBodies Ai (fst (mutatorMap name)) (fst s) x),
-               fst (PMutatorMethodBodies Bi (snd (mutatorMap name)) (snd s) x)),
-              0);
-        PObserverMethodBodies name :=
-          match observerMap name with
-            | inl name'
-              => match PObserverMethodBodies Ai name' with
-                   | Some body => Some (fun s x
-                                        => let sy := body (fst s) x in
-                                           ((fst sy, snd s), snd sy))
-                   | None => None
-                 end
-            | inr name'
-              => match PObserverMethodBodies Bi name' with
-                   | Some body => Some (fun s x
-                                        => let sy := body (snd s) x in
-                                           ((fst s, fst sy), snd sy))
-                   | None => None
-                 end
-          end
-      |};
-    repeat match goal with
-             | _ => intro
-             | _ => progress simpl in *
-             | [ idx : mutatorIndex, H : PRepInv Ai _ _ /\ PRepInv Bi _ _, x : nat |- _ ]
-               => generalize (PMutatorMethodsCorrect Ai (fst (mutatorMap idx)) _ _ (proj1 H) x);
-                 generalize (PMutatorMethodsCorrect Bi (snd (mutatorMap idx)) _ _ (proj2 H) x);
-                 destruct (mutatorMap idx), H; simpl in *;
-                 clear idx;
-                 progress repeat destruct PMutatorMethodBodies;
-                 simpl in *;
-                 firstorder; subst
-             | [ idx : ObserverIndex _ |- appcontext[PRepInv ?Ai] ]
-               => unique_pose (PObserverMethodsCorrect Ai idx)
-             | [ |- appcontext[match PObserverMethodBodies ?i ?name with _ => _ end] ]
-               => destruct (PObserverMethodBodies i name);
-                 simpl in *;
-                 unfold observerMethodCorrect in *;
-                 split_and;
-                 intros;
-                 split;
-                 try solve [ intuition ]
-             | [ idx : observerIndex |- _ ]
-               => destruct (observerMap idx) as [idx'|idx']; clear idx
-             | _ => eexists (_, _)
-             | _ => progress (repeat esplit; try eassumption)
-             | _ => apply PObserverMethodsCorrect
-             | _ => progress firstorder intuition
-           end.
-  Defined.
-End pairedPartial.
+    Variable mutatorIndex : Type.
+    Variable observerIndex : Type.
+    Variable mutatorMap : mutatorIndex -> MutatorIndex A * MutatorIndex B.
+    Variable observerMap : observerIndex -> ObserverIndex A + ObserverIndex B.
 
-Section prodPartial.
-  Variable model : Type.
-  Variables AMutIndex BMutIndex AObsIndex BObsIndex : Type.
-  Variable AMutSpec : AMutIndex -> mutatorMethodSpec model.
-  Variable BMutSpec : BMutIndex -> mutatorMethodSpec model.
-  Variable AObsSpec : AObsIndex -> observerMethodSpec model.
-  Variable BObsSpec : BObsIndex -> observerMethodSpec model.
+    (** Now we show how to implement it. *)
+    Variable Ai : PartialADTimpl A.
+    Variable Bi : PartialADTimpl B.
 
-  Let A := {| Model := model;
-              MutatorMethodSpecs := AMutSpec;
-              ObserverMethodSpecs := AObsSpec |}.
-  Let B := {| Model := model;
-              MutatorMethodSpecs := BMutSpec;
-              ObserverMethodSpecs := BObsSpec |}.
+    Definition pairedPartialImpl
+    : PartialADTimpl (pairedADT A B mutatorMap observerMap).
+    Proof.
+      refine {|
+          PState := PState Ai * PState Bi;
+          PRepInv := fun (m : Model (pairedADT A B mutatorMap observerMap)) s
+                     => PRepInv Ai (fst m) (fst s)
+                        /\ PRepInv Bi (snd m) (snd s);
+          PMutatorMethodBodies name :=
+            fun s x
+            => (A_val <- PMutatorMethodBodies Ai (fst (mutatorMap name)) (fst s) x;
+                B_val <- PMutatorMethodBodies Bi (snd (mutatorMap name)) (snd s) x;
+                ret ((fst A_val, fst B_val), 0))%comp;
+          PObserverMethodBodies name :=
+            match observerMap name with
+              | inl name'
+                => match PObserverMethodBodies Ai name' with
+                     | Some body => Some (fun s x
+                                          => (sy <- body (fst s) x;
+                                              ret ((fst sy, snd s), snd sy))%comp)
+                     | None => None
+                   end
+              | inr name'
+                => match PObserverMethodBodies Bi name' with
+                     | Some body => Some (fun s x
+                                          => (sy <- body (snd s) x;
+                                              ret ((fst s, fst sy), snd sy))%comp)
+                     | None => None
+                   end
+            end
+        |};
+      abstract (
+          repeat intro;
+          unfold observerMethodCorrect; simpl;
+          destruct_sum_in_match;
+          simpl in *;
+            repeat match goal with
+                     | [ |- appcontext[PObserverMethodBodies ?Ai ?x] ]
+                       => generalize (PObserverMethodsCorrect Ai x);
+                     destruct (PObserverMethodBodies Ai x)
+                   end;
+          p_impl_t
+        ).
+    Defined.
+  End pairedPartial.
 
-  Variable mutatorIndex : Type.
-  Variable observerIndex : Type.
-  Variable mutatorMap : mutatorIndex -> MutatorIndex A * MutatorIndex B.
-  Variable observerMap : observerIndex -> ObserverIndex A + ObserverIndex B.
+  Section prodPartial.
+    Variable model : Type.
+    Variables AMutIndex BMutIndex AObsIndex BObsIndex : Type.
+    Variable AMutSpec : AMutIndex -> mutatorMethodSpec model.
+    Variable BMutSpec : BMutIndex -> mutatorMethodSpec model.
+    Variable AObsSpec : AObsIndex -> observerMethodSpec model.
+    Variable BObsSpec : BObsIndex -> observerMethodSpec model.
 
-  Local Notation prodADT := (prodADT AMutSpec BMutSpec
-                                     AObsSpec BObsSpec
-                                     mutatorMap
-                                     observerMap).
+    Let A := {| Model := model;
+                MutatorMethodSpecs := AMutSpec;
+                ObserverMethodSpecs := AObsSpec |}.
+    Let B := {| Model := model;
+                MutatorMethodSpecs := BMutSpec;
+                ObserverMethodSpecs := BObsSpec |}.
 
-  (** Now we show how to implement it. *)
-  Variable Ai : PartialADTimpl A.
-  Variable Bi : PartialADTimpl B.
+    Variable mutatorIndex : Type.
+    Variable observerIndex : Type.
+    Variable mutatorMap : mutatorIndex -> MutatorIndex A * MutatorIndex B.
+    Variable observerMap : observerIndex -> ObserverIndex A + ObserverIndex B.
 
-  Local Hint Extern 1 (@ex (_ * _) _) => eexists (_, _).
+    Local Notation prodADT := (prodADT AMutSpec BMutSpec
+                                       AObsSpec BObsSpec
+                                       mutatorMap
+                                       observerMap).
 
-  Hypothesis mutators_match
-  : forall idx,
+    (** Now we show how to implement it. *)
+    Variable Ai : PartialADTimpl A.
+    Variable Bi : PartialADTimpl B.
+
+    Local Hint Extern 1 (@ex (_ * _) _) => eexists (_, _).
+
+    Hypothesis mutators_match
+    : forall idx,
       forall m x m' m'',
         AMutSpec (fst (mutatorMap idx)) m x m'
         -> BMutSpec (snd (mutatorMap idx)) m x m''
         -> m' = m''.
 
-  Local Hint Extern 1 => symmetry.
+    Local Hint Extern 1 => apply symmetry.
 
-  Definition prodPartialImpl : PartialADTimpl prodADT.
-  Proof.
-    refine {|
-        PState := PState Ai * PState Bi;
-        PRepInv := fun (m : Model prodADT) s
-                   => PRepInv Ai m (fst s)
-                      /\ PRepInv Bi m (snd s);
-        PMutatorMethodBodies idx :=
-          fun s x =>
-            let s1 := fst (PMutatorMethodBodies Ai (fst (mutatorMap idx)) (fst s) x) in
-            let s2 := fst (PMutatorMethodBodies Bi (snd (mutatorMap idx)) (snd s) x) in
-            ((s1, s2), 0);
-        PObserverMethodBodies idx :=
-          match observerMap idx with
-            | inl idx' =>
-              match PObserverMethodBodies Ai idx' with
-                | Some body => Some (fun s x =>
-                                       let s'y := body (fst s) x in
-                                       ((fst s'y, snd s), snd s'y))
-                | None => None
-              end
-            | inr idx' =>
-              match PObserverMethodBodies Bi idx' with
-                | Some body => Some (fun s x =>
-                                       let s'y := body (snd s) x in
-                                       ((fst s, fst s'y), snd s'y))
-                | None => None
-              end
-          end
-      |};
-    intro idx;
-    try (assert (MM := mutators_match idx));
-    repeat intro;
-    simpl in *;
-    match goal with
-      | [ |- appcontext[mutatorMap ?idx] ]
-        => destruct (mutatorMap idx); clear idx
-      | [ |- appcontext[observerMap ?idx] ]
-        => destruct (observerMap idx); clear idx
-    end;
-    simpl in *;
-    repeat split;
-    try match goal with
-          | [ |- appcontext[PObserverMethodBodies ?i ?idx] ]
-            => pose proof (PObserverMethodsCorrect i idx);
-              destruct (PObserverMethodBodies i idx)
-        end;
-    simpl in *;
-    unfold observerMethodCorrect in *;
-    split_and;
-    simpl in *;
-    intuition.
-    - edestruct (PMutatorMethodsCorrect Ai); try eassumption.
-      edestruct (PMutatorMethodsCorrect Bi); try eassumption.
-      simpl in *.
-      intuition.
-      match goal with
-        | [ AM : AMutSpec _ _ _ _, BM : BMutSpec _ _ _ _ |- _ ]
-          => specialize (MM _ _ _ _ AM BM); subst
-      end.
-      repeat esplit; eassumption.
-  Defined.
-End prodPartial.
+    Definition prodPartialImpl : PartialADTimpl prodADT.
+    Proof.
+      refine {|
+          PState := PState Ai * PState Bi;
+          PRepInv := fun (m : Model prodADT) s
+                     => PRepInv Ai m (fst s)
+                        /\ PRepInv Bi m (snd s);
+          PMutatorMethodBodies idx :=
+            fun s x =>
+              (s1 <- PMutatorMethodBodies Ai (fst (mutatorMap idx)) (fst s) x;
+               s2 <- PMutatorMethodBodies Bi (snd (mutatorMap idx)) (snd s) x;
+               ret ((fst s1, fst s2), 0))%comp;
+          PObserverMethodBodies idx :=
+            match observerMap idx with
+              | inl idx' =>
+                match PObserverMethodBodies Ai idx' with
+                  | Some body => Some (fun s x =>
+                                         (s'y <- body (fst s) x;
+                                          ret ((fst s'y, snd s), snd s'y))%comp)
+                  | None => None
+                end
+              | inr idx' =>
+                match PObserverMethodBodies Bi idx' with
+                  | Some body => Some (fun s x =>
+                                         (s'y <- body (snd s) x;
+                                          ret ((fst s, fst s'y), snd s'y))%comp)
+                  | None => None
+                end
+            end
+        |};
+      abstract (
+          intro idx;
+          try (assert (MM := mutators_match idx));
+          repeat intro;
+          unfold observerMethodCorrect; simpl;
+          destruct_sum_in_match;
+          simpl in *;
+            repeat match goal with
+                     | [ |- appcontext[PObserverMethodBodies ?Ai ?x] ]
+                       => generalize (PObserverMethodsCorrect Ai x);
+                     destruct (PObserverMethodBodies Ai x)
+                   end;
+          p_impl_t';
+          try match goal with
+                | [ AM : AMutSpec _ _ _ _, BM : BMutSpec _ _ _ _ |- _ ]
+                  => specialize (MM _ _ _ _ AM BM); subst
+              end;
+          p_impl_t
+        ).
+    Defined.
+  End prodPartial.
 
 
-(** A transformation (approximately, injection) from one ADT to another *)
+  (** A transformation (approximately, injection) from one ADT to another *)
 
-Section injPartial.
-  Variables A B : ADT.
-  (** Let's compose these two ADTs. *)
+  Section injPartial.
+    Variables A B : ADT.
+    (** Let's compose these two ADTs. *)
 
-  Variable AtoB : Model A -> Model B.
-  Variable BtoA : Model B -> Model A.
-  Variable mutatorMap : MutatorIndex B -> MutatorIndex A.
-  Variable observerMap : ObserverIndex B -> ObserverIndex A.
-  Hypothesis mutatorSpecMap
-  : forall idx m x m',
-      MutatorMethodSpecs A (mutatorMap idx) (BtoA m) x m'
-      -> exists m'',
-           m' = BtoA m''
-           /\ MutatorMethodSpecs B idx m x m''.
-  Hypothesis observerSpecMap
-  : forall idx m x y,
-      ObserverMethodSpecs A (observerMap idx) (BtoA m) x y
-      -> ObserverMethodSpecs B idx m x y.
-
-
-  Variable Ai : PartialADTimpl A.
-
-  Definition injPartialImpl : PartialADTimpl B.
-  Proof.
-    refine {|
-        PState := PState Ai;
-        PRepInv := fun (m : Model B) s
-                  => PRepInv Ai (BtoA m) s;
-        PMutatorMethodBodies name := PMutatorMethodBodies Ai (mutatorMap name);
-        PObserverMethodBodies name := PObserverMethodBodies Ai (observerMap name)
-      |};
-    intro idx;
-    let H := fresh in
-    first [ assert (H := PMutatorMethodsCorrect Ai (mutatorMap idx))
-          | assert (H := PObserverMethodsCorrect Ai (observerMap idx));
-            edestruct PObserverMethodBodies; trivial ];
-      let inv := fresh in
-      let x := fresh in
-      intros ? ? inv x;
-        specialize (H _ _ inv x);
-        simpl in *;
-        intuition;
-        let m := fresh "m" in
-        destruct H as [m H];
-          split_and.
-    let H0 := match goal with
-                | [ H : _ |- _ ] => constr:(@mutatorSpecMap _ _ _ _ H)
-              end in
-    let m := fresh "m" in
-    destruct H0 as [m ?];
-      split_and;
-      exists m;
-      subst;
-      intuition.
-  Defined.
-End injPartial.
+    Variable AtoB : Model A -> Model B.
+    Variable BtoA : Model B -> Model A.
+    Variable mutatorMap : MutatorIndex B -> MutatorIndex A.
+    Variable observerMap : ObserverIndex B -> ObserverIndex A.
+    Hypothesis mutatorSpecMap
+    : forall idx m x m',
+        MutatorMethodSpecs A (mutatorMap idx) (BtoA m) x m'
+        -> exists m'',
+             m' = BtoA m''
+             /\ MutatorMethodSpecs B idx m x m''.
+    Hypothesis observerSpecMap
+    : forall idx m x y,
+        ObserverMethodSpecs A (observerMap idx) (BtoA m) x y
+        -> ObserverMethodSpecs B idx m x y.
 
 
-(** Notes: it should be m' = BtoA m' m'' in mutators_match; actually we probably want [mutators_match : forall idx m x m', MutatorMethodSpecs B (Ms idx) (AtoB m) x m' -> exists m'', AtoB m'' = m'] *)
-Lemma add_component A B (Bimpl : ADTimpl B) later
-  (Is : ObserverIndex A -> ObserverIndex B + later)
-  (unlater : later -> ObserverIndex A)
-  (Ms : MutatorIndex A -> MutatorIndex B)
-  (AtoB : Model A -> Model B)
-  (mutators_match : forall idx,
-    forall m x m',
-      MutatorMethodSpecs B (Ms idx) (AtoB m) x m'
-      -> exists m'', m' = AtoB m''
-                     /\ MutatorMethodSpecs A idx m x m'')
-  (mutators_match_hammer : forall idx,
-    forall m x m' m'',
-      MutatorMethodSpecs B (Ms idx) (AtoB m) x m'
-      -> MutatorMethodSpecs A idx m x m''
-      -> m' = AtoB m'')
-  (observers_match : forall idx,
-    match Is idx with
-      | inr _ => True
-      | inl idx' =>
-        forall m x y,
-          ObserverMethodSpecs A idx m x y
-          <-> ObserverMethodSpecs B idx' (AtoB m) x y
-    end)
-  (almost_adjunction : forall idx l, Is idx = inr l -> idx = unlater l)
+    Variable Ai : PartialADTimpl A.
+
+    Definition injPartialImpl : PartialADTimpl B.
+    Proof.
+      refine {|
+          PState := PState Ai;
+          PRepInv := fun (m : Model B) s
+                     => PRepInv Ai (BtoA m) s;
+          PMutatorMethodBodies name := PMutatorMethodBodies Ai (mutatorMap name);
+          PObserverMethodBodies name := PObserverMethodBodies Ai (observerMap name)
+        |};
+      abstract (
+          repeat intro;
+          unfold observerMethodCorrect in *; simpl;
+          destruct_sum_in_match;
+          simpl in *;
+            repeat match goal with
+                     | [ |- appcontext[PObserverMethodBodies ?Ai ?x] ]
+                       => generalize (PObserverMethodsCorrect Ai x);
+                     destruct (PObserverMethodBodies Ai x)
+                   end;
+          unfold observerMethodCorrect in *; simpl;
+          p_impl_t';
+          try solve [ p_impl_t ];
+          edestruct mutatorSpecMap; try eassumption;
+          p_impl_t
+        ).
+    Defined.
+  End injPartial.
+
+
+  (** Notes: it should be m' = BtoA m' m'' in mutators_match; actually we probably want [mutators_match : forall idx m x m', MutatorMethodSpecs B (Ms idx) (AtoB m) x m' -> exists m'', AtoB m'' = m'] *)
+  Lemma add_component A B (Bimpl : ADTimpl B) later
+        (Is : ObserverIndex A -> ObserverIndex B + later)
+        (unlater : later -> ObserverIndex A)
+        (Ms : MutatorIndex A -> MutatorIndex B)
+        (AtoB : Model A -> Model B)
+        (mutators_match : forall idx,
+                          forall m x m',
+                            MutatorMethodSpecs B (Ms idx) (AtoB m) x m'
+                            -> exists m'', m' = AtoB m''
+                                           /\ MutatorMethodSpecs A idx m x m'')
+        (mutators_match_hammer : forall idx,
+                                 forall m x m' m'',
+                                   MutatorMethodSpecs B (Ms idx) (AtoB m) x m'
+                                   -> MutatorMethodSpecs A idx m x m''
+                                   -> m' = AtoB m'')
+        (observers_match : forall idx,
+                             match Is idx with
+                               | inr _ => True
+                               | inl idx' =>
+                                 forall m x y,
+                                   ObserverMethodSpecs A idx m x y
+                                   <-> ObserverMethodSpecs B idx' (AtoB m) x y
+                             end)
+        (almost_adjunction : forall idx l, Is idx = inr l -> idx = unlater l)
   : PartialADTimpl {| Model := Model A;
-    MutatorIndex := MutatorIndex A;
-    ObserverIndex := later;
-    MutatorMethodSpecs := MutatorMethodSpecs A;
-    ObserverMethodSpecs i := ObserverMethodSpecs A (unlater i)
-  |}
-  -> PartialADTimpl A.
-Proof.
-  intro Aimpl.
-  pose (Bimpl : PartialADTimpl _) as Bimpl'.
-  Print Implicit injPartialImpl.
-  let A' := match type of Aimpl with PartialADTimpl ?A' => constr:(A') end in
-  pose (@pairedPartialImpl
-          A' B
-          (MutatorIndex A)
-          (ObserverIndex A)
-          (fun idx => (idx, Ms idx))
-          (fun idx => match Is idx with
-                        | inl idx' => inr idx'
-                        | inr idx' => inl idx'
-                      end)
-          Aimpl
-          Bimpl')
-    as ABimpl;
-    let AB := match type of ABimpl with PartialADTimpl ?AB => constr:(AB) end in
-    apply (fun g h =>
-            @injPartialImpl
-              AB A
-              (fun a => (a, AtoB a))
-              (fun x => x)
-              (fun x => x)
-              g h
-              ABimpl);
-    simpl in *;
-    try solve [ intuition ];
-    [
-    | solve [ intros idx; intros;
-              specialize (observers_match idx);
-              repeat match goal with
-                       | [ H : appcontext[Is idx] |- _ ] => revert H
-                     end;
-              case_eq (Is idx);
-              intros;
-              split_iff;
-              rewrite ?Htos' in *;
-              intuition;
-              erewrite <- almost_adjunction in * by eassumption; trivial
-    ] ].
-  - intros idx m x [m'A m'B] ?; simpl in *.
-    intuition.
-    f_equal.
-    esplit; intuition eauto; f_equal.
-    eapply mutators_match_hammer; try eassumption.
-Defined.
+                      MutatorIndex := MutatorIndex A;
+                      ObserverIndex := later;
+                      MutatorMethodSpecs := MutatorMethodSpecs A;
+                      ObserverMethodSpecs i := ObserverMethodSpecs A (unlater i)
+                   |}
+    -> PartialADTimpl A.
+  Proof.
+    intro Aimpl.
+    pose (Bimpl : PartialADTimpl _) as Bimpl'.
+    Print Implicit injPartialImpl.
+    let A' := match type of Aimpl with PartialADTimpl ?A' => constr:(A') end in
+    pose (@pairedPartialImpl
+            A' B
+            (MutatorIndex A)
+            (ObserverIndex A)
+            (fun idx => (idx, Ms idx))
+            (fun idx => match Is idx with
+                          | inl idx' => inr idx'
+                          | inr idx' => inl idx'
+                        end)
+            Aimpl
+            Bimpl')
+      as ABimpl;
+      let AB := match type of ABimpl with PartialADTimpl ?AB => constr:(AB) end in
+      apply (fun g h =>
+               @injPartialImpl
+                 AB A
+                 (fun a => (a, AtoB a))
+                 (fun x => x)
+                 (fun x => x)
+                 g h
+                 ABimpl);
+        simpl in *;
+        try solve [ intuition ];
+        [
+        | solve [ intros idx; intros;
+                  specialize (observers_match idx);
+                  repeat match goal with
+                           | [ H : appcontext[Is idx] |- _ ] => revert H
+                         end;
+                  case_eq (Is idx);
+                  intros;
+                  split_iff;
+                  rewrite ?Htos' in *;
+                  intuition;
+                  erewrite <- almost_adjunction in * by eassumption; trivial
+        ] ].
+    - intros idx m x [m'A m'B] ?; simpl in *.
+      intuition.
+      f_equal.
+      esplit; intuition eauto; f_equal.
+      eapply mutators_match_hammer; try eassumption.
+  Defined.
 
-Lemma no_observers (A : ADT) (Hreally : ObserverIndex A -> False)
-  (Himplementable : forall idx m x,
-    exists m', MutatorMethodSpecs A idx m x m')
+  Lemma no_observers (A : ADT) (Hreally : ObserverIndex A -> False)
+        (Himplementable : forall idx m x,
+                          exists m', MutatorMethodSpecs A idx m x m')
   : PartialADTimpl A.
-  refine {| PState := unit;
-    PRepInv := fun _ _ => True;
-    PMutatorMethodBodies := fun _ _ _ => (tt, 0);
-    PObserverMethodBodies := fun _ => None
-  |}; auto.
+    refine {| PState := unit;
+              PRepInv := fun _ _ => True;
+              PMutatorMethodBodies := fun _ _ _ => (ret (tt, 0))%comp;
+              PObserverMethodBodies := fun _ => None
+           |}; auto.
+    repeat intro; simpl in *.
+    inversion_computes_to; subst; simpl.
+    edestruct Himplementable.
+    repeat esplit; eassumption.
+  Defined.
 
-  intro.
-  hnf; simpl; intros.
-  edestruct Himplementable.
-  eauto.
-Defined.
+  Goal PartialADTimpl NatSumProd_spec.
+  Proof.
+    pose proof (add_component NatSumProd_spec
+                              (NatSumI 0)
+                              (later := unit)).
 
-Goal PartialADTimpl NatSumProd_spec.
-Proof.
-  pose proof (add_component NatSumProd_spec
-    (NatSumI 0)
-    (later := unit)).
-
-  eapply (add_component NatSumProd_spec
-    (NatSumI 0)
-    (later := unit)
-    (fun x => x)
-    (fun x => inr x)
-    (fun x => x) (fun x => x));
-  auto.
-  - simpl.
-    simpl; intros.
-    eexists; repeat esplit; trivial.
-  - destruct idx; simpl.
-    intros.
-    Require Import FunctionalExtensionality.
-    extensionality n.
-    rewrite H, H0; auto.
-
-  - destruct idx; intuition.
-
-  - let A := match goal with |- PartialADTimpl ?A => constr:(A) end in
-    eapply (add_component A
-                          (NatProdI 1) (later := Empty_set)
-                          (fun x => inl x)
-                          (fun x => match x with end)
+    eapply (add_component NatSumProd_spec
+                          (NatSumI 0)
+                          (later := unit)
                           (fun x => x)
-                          (fun x => x));
-      simpl; auto.
-    + simpl.
+                          (fun x => inr x)
+                          (fun x => x) (fun x => x));
+      auto.
+    - simpl.
       simpl; intros.
       eexists; repeat esplit; trivial.
-    + intros.
+    - destruct idx; simpl.
+      intros.
       Require Import FunctionalExtensionality.
       extensionality n.
       rewrite H, H0; auto.
 
-    + tauto.
-    + destruct l.
+    - destruct idx; intuition.
 
-    + apply no_observers; simpl; intros.
-      destruct H.
-      exists (fun k => if eq_nat_dec x k then S (m k) else m k).
-      auto.
-Defined.
+    - let A := match goal with |- PartialADTimpl ?A => constr:(A) end in
+      eapply (add_component A
+                            (NatProdI 1) (later := Empty_set)
+                            (fun x => inl x)
+                            (fun x => match x with end)
+                            (fun x => x)
+                            (fun x => x));
+        simpl; auto.
+      + simpl.
+        simpl; intros.
+        eexists; repeat esplit; trivial.
+      + intros.
+        Require Import FunctionalExtensionality.
+        extensionality n.
+        rewrite H, H0; auto.
 
+      + tauto.
+      + destruct l.
 
-Existing Class ADTimpl.
-Hint Extern 1 (ADTimpl _) => eapply NatLowerI : typeclass_instances.
-Hint Extern 1 (ADTimpl _) => eapply NatUpperI : typeclass_instances.
-Hint Extern 1 (ADTimpl _) => eapply NatSumI : typeclass_instances.
-Hint Extern 1 (ADTimpl _) => eapply NatProdI : typeclass_instances.
-Hint Extern 2 (ADTimpl _) => eapply pairedImpl : typeclass_instances.
+      + apply no_observers; simpl; intros.
+        destruct H.
+        exists (fun k => if eq_nat_dec x k then S (m k) else m k).
+        auto.
+  Defined.
 
-Record refine (from to : ADT) :=
-  {
-    MakeImpl : ADTimpl from -> ADTimpl to;
-    MapMutator : MutatorIndex to -> option (MutatorIndex from);
-    MapObserver : ObserverIndex to -> option (ObserverIndex from)
-  }.
+(*
+  Existing Class ADTimpl.
+  Hint Extern 1 (ADTimpl _) => eapply NatLowerI : typeclass_instances.
+  Hint Extern 1 (ADTimpl _) => eapply NatUpperI : typeclass_instances.
+  Hint Extern 1 (ADTimpl _) => eapply NatSumI : typeclass_instances.
+  Hint Extern 1 (ADTimpl _) => eapply NatProdI : typeclass_instances.
+  Hint Extern 2 (ADTimpl _) => eapply pairedImpl : typeclass_instances.
 
-Definition empty :=
-  {|
-    Model := unit;
-    MutatorIndex := Empty_set;
-    ObserverIndex := Empty_set;
+  Record refine (from_ to : ADT) :=
+    {
+      MakeImpl : ADTimpl from_ -> ADTimpl to;
+      MapMutator : MutatorIndex to -> option (MutatorIndex from_);
+      MapObserver : ObserverIndex to -> option (ObserverIndex from_)
+    }.
 
-    MutatorMethodSpecs := fun x : Empty_set => match x with end;
-    ObserverMethodSpecs := fun x : Empty_set => match x with end
-  |}.
-
-Definition emptyI : ADTimpl empty :=
-  {|
-    State := unit;
-    RepInv := fun _ _ => True;
-    MutatorMethodBodies := fun x : MutatorIndex empty => match x with end;
-    ObserverMethodBodies := fun x : Empty_set => match x with end;
-    MutatorMethodsCorrect := fun x : Empty_set => match x with end;
-    ObserverMethodsCorrect := fun x : Empty_set => match x with end
-  |}.
-
-
-Definition ADTimpl' (to : ADT) := refine empty to.
-
-Theorem finish : forall to (ai' : ADTimpl' to), ADTimpl to.
-  destruct 1; eauto using emptyI.
-Defined.
-
-Definition easy from : refine from from :=
-  {|
-    MakeImpl := fun x => x;
-    MapMutator := fun x => Some x;
-    MapObserver := fun x => Some x
-  |}.
-
-Section refinePaired.
-  Variables from new : ADT.
-
-  Variable mutatorIndex : Type.
-  Variable observerIndex : Type.
-  Variable mutatorMap : mutatorIndex -> MutatorIndex from * MutatorIndex new.
-  Variable observerMap : observerIndex -> ObserverIndex from + ObserverIndex new.
-
-  Definition refinePaired to (newI : ADTimpl new)
-  : refine (pairedADT from new mutatorMap observerMap) to
-    -> refine from to
-    := fun r =>
-         {| MakeImpl fromI := MakeImpl r (pairedImpl _ _ fromI newI);
-            MapMutator toIndex :=
-              match MapMutator r toIndex with
-                | None => None
-                | Some idx => Some (fst (mutatorMap idx))
-              end;
-            MapObserver toIndex :=
-              match MapObserver r toIndex with
-                | None => None
-                | Some idx => match observerMap idx with
-                                | inl idx' => Some idx'
-                                | inr idx' => None
-                              end
-              end
-         |}.
-End refinePaired.
-
-Goal ADTimpl NatSumProd_spec.
-Proof.
-  eapply finish.
-  unfold NatSumProd_spec.
-  eapply refinePaired.
-
-
-Section pairedAlgorithmic.
-  Variables A B : ADT.
-
-  Variable mutatorIndex : Type.
-  Variable observerIndex : Type.
-  Variable mutatorMap : mutatorIndex -> MutatorIndex A * MutatorIndex B.
-  Variable observerMap : observerIndex -> ObserverIndex A + ObserverIndex B.
-
-  (** The composed ADT *)
-  Definition pairedADT :=
+  Definition empty :=
     {|
-      Model := Model A * Model B;
-      MutatorIndex := mutatorIndex;
-      ObserverIndex := observerIndex;
-      MutatorMethodSpecs idx :=
-        let s := mutatorMap idx in
-        fun m x m' => MutatorMethodSpecs A (fst s) (fst m) x (fst m')
-                      /\ MutatorMethodSpecs B (snd s) (snd m) x (snd m');
-      ObserverMethodSpecs idx :=
-        fun m x y => match observerMap idx with
-                       | inl idx' => ObserverMethodSpecs A idx' (fst m) x y
-                       | inr idx' => ObserverMethodSpecs B idx' (snd m) x y
-                     end
+      Model := unit;
+      MutatorIndex := Empty_set;
+      ObserverIndex := Empty_set;
+
+      MutatorMethodSpecs := fun x : Empty_set => match x with end;
+      ObserverMethodSpecs := fun x : Empty_set => match x with end
     |}.
 
-  (** Now we show how to implement it. *)
-  Variable Ai : ADTimpl A.
-  Variable Bi : ADTimpl B.
-    ADTimpl a1
-    -> ADTimpl a2
-    -> ADTimpl a.
+  Definition emptyI : ADTimpl empty :=
+    {|
+      State := unit;
+      RepInv := fun _ _ => True;
+      MutatorMethodBodies := fun x : MutatorIndex empty => match x with end;
+      ObserverMethodBodies := fun x : Empty_set => match x with end;
+      MutatorMethodsCorrect := fun x : Empty_set => match x with end;
+      ObserverMethodsCorrect := fun x : Empty_set => match x with end
+    |}.
 
 
-Typeclasses eauto := debug.
-Goal ADTimpl NatSumProd_spec.
-  unfold NatSumProd_spec.
+  Definition ADTimpl' (to : ADT) := refine empty to.
+
+  Theorem finish : forall to (ai' : ADTimpl' to), ADTimpl to.
+    destruct 1; eauto using emptyI.
+  Defined.
+
+  Definition easy from_ : refine from_ from_ :=
+    {|
+      MakeImpl := fun x => x;
+      MapMutator := fun x => Some x;
+      MapObserver := fun x => Some x
+    |}.
+
+  Section refinePaired.
+    Variables from_ new : ADT.
+
+    Variable mutatorIndex : Type.
+    Variable observerIndex : Type.
+    Variable mutatorMap : mutatorIndex -> MutatorIndex from_ * MutatorIndex new.
+    Variable observerMap : observerIndex -> ObserverIndex from_ + ObserverIndex new.
+
+    Definition refinePaired to (newI : ADTimpl new)
+    : refine (pairedADT from_ new mutatorMap observerMap) to
+      -> refine from_ to
+      := fun r =>
+           {| MakeImpl fromI := MakeImpl r (pairedImpl _ _ fromI newI);
+              MapMutator toIndex :=
+                match MapMutator r toIndex with
+                  | None => None
+                  | Some idx => Some (fst (mutatorMap idx))
+                end;
+              MapObserver toIndex :=
+                match MapObserver r toIndex with
+                  | None => None
+                  | Some idx => match observerMap idx with
+                                  | inl idx' => Some idx'
+                                  | inr idx' => None
+                                end
+                end
+           |}.
+  End refinePaired.
+
+  Goal ADTimpl NatSumProd_spec.
+  Proof.
+    eapply finish.
+    unfold NatSumProd_spec.
+    eapply refinePaired.
+
+(*
+    Section pairedAlgorithmic.
+      Variables A B : ADT.
+
+      Variable mutatorIndex : Type.
+      Variable observerIndex : Type.
+      Variable mutatorMap : mutatorIndex -> MutatorIndex A * MutatorIndex B.
+      Variable observerMap : observerIndex -> ObserverIndex A + ObserverIndex B.
+
+      (** The composed ADT *)
+      Definition pairedADT :=
+        {|
+          Model := Model A * Model B;
+          MutatorIndex := mutatorIndex;
+          ObserverIndex := observerIndex;
+          MutatorMethodSpecs idx :=
+            let s := mutatorMap idx in
+            fun m x m' => MutatorMethodSpecs A (fst s) (fst m) x (fst m')
+                          /\ MutatorMethodSpecs B (snd s) (snd m) x (snd m');
+          ObserverMethodSpecs idx :=
+            fun m x y => match observerMap idx with
+                           | inl idx' => ObserverMethodSpecs A idx' (fst m) x y
+                           | inr idx' => ObserverMethodSpecs B idx' (snd m) x y
+                         end
+        |}.
+
+      (** Now we show how to implement it. *)
+      Variable Ai : ADTimpl A.
+      Variable Bi : ADTimpl B.
+      ADTimpl a1
+      -> ADTimpl a2
+      -> ADTimpl a.
 
 
-
-unfold NatSumProd_spec.
-let f := lazymatch goal with |- ADTimpl {| MutatorMethodSpecs := ?f |} => constr:(f) end in
-let f' := constr:(fun idx ma mb x m'a m'b => f idx (ma, mb) x (m'a, m'b)) in
-let f'' := (eval simpl in f') in
-let f0f1 := lazymatch f'' with
-              | (fun idx ma mb x m'a m'b => @?f0 idx ma x m'a /\ @?f1 idx mb x m'b)
-                => constr:((f0, f1))
-            end in
-let AMutatorMethodSpecs := constr:(fst f0f1) in
-let BMutatorMethodSpecs := constr:(snd f0f1) in
-let fObs := match goal with |- ADTimpl {| ObserverMethodSpecs := ?f |} => constr:(f) end in
-let f'Obs := constr:(fun idx ma mb x y => fObs idx (ma, mb) x y) in
-let f''Obs := (eval simpl in f'Obs) in
-let f0f1Obs := lazymatch f''Obs with
-                 | (fun idx ma mb x y =>
-                      match idx with
-                        | inl idx' => @?f0 ma x y idx'
-                        | inr idx' => @?f1 mb x y idx'
-                      end)
-                   => constr:((f0, f1))
-               end in
-let AObserverMethodSpecs := constr:(fst f0f1Obs) in
-let BObserverMethodSpecs := constr:(snd f0f1Obs) in
-lazymatch goal with
-  | [ |- ADTimpl
-           {|
-             Model := ?AModel * ?BModel;
-             MutatorIndex := ?mutatorIndex;
-             ObserverIndex := ?observerIndex
-           |} ]
-    => pose proof (@pairedImpl
-                     (@Build_ADT AModel _ _ AMutatorMethodSpecs (fun idx' ma x y => AObserverMethodSpecs ma x y idx'))
-                     (@Build_ADT BModel _ _ BMutatorMethodSpecs (fun idx' mb x y => BObserverMethodSpecs mb x y idx'))
-                     mutatorIndex
-                     observerIndex
-                     (fun x => (x, x))
-                     (fun x => x));
-      unfold pairedADT in *; simpl in *
-end.
-    eapply X;
-    eauto with typeclass_instances.
-Defined.
-
-Definition NatLowerUpper_sortOf (s : string) :=
-  if string_dec s "add"
-    then Mutator
-    else if string_dec s "lowerBound"
-      then ObserverA
-      else if string_dec s "upperBound"
-        then ObserverB
-        else Dummy.
-
-Definition NatLowerUpperPair : ADT
-  := pairedADT (NatLower "add" "lowerBound")
-               (NatUpper "add" "upperBound")
-               NatLowerUpper_sortOf.
-Definition NatLowerUpperProd : ADT
-  := prodADT (MethodSpecs (NatLower "add" "lowerBound"))
-             (MethodSpecs (NatUpper "add" "upperBound"))
-             NatLowerUpper_sortOf.
-
-Local Ltac pair_I_tac :=
-  repeat match goal with
-           | _ => intro
-           | _ => progress simpl in *
-           | [ |- context[if ?E then _ else _ ] ] => destruct E; subst
-         end;
-  simpl; unfold mutator, observer; simpl; instantiate; firstorder (subst; eauto).
-
-Definition NatLowerUpperPairI : ADTimpl NatLowerUpperPair.
-  refine (pairedImpl NatLowerUpper_sortOf
-                     (NatLowerI "add" "lowerBound" I)
-                     (NatUpperI "add" "upperBound" I)
-                     _);
-  unfold NatLowerUpper_sortOf.
-  abstract pair_I_tac.
-Defined.
-
-Definition NatLowerUpperProdI : ADTimpl NatLowerUpperProd.
-  refine (prodImpl NatLowerUpper_sortOf
-                   (NatLowerI "add" "lowerBound" I)
-                   (NatUpperI "add" "upperBound" I)
-                   _
-                   _);
-  unfold NatLowerUpper_sortOf;
-  abstract pair_I_tac.
-Defined.
+      Typeclasses eauto := debug.
+      Goal ADTimpl NatSumProd_spec.
+        unfold NatSumProd_spec.
 
 
 
-Definition s0pair : State NatLowerUpperPairI := (Some 10, Some 100).
-Definition s1pair := fst (MethodBodies NatLowerUpperPairI "add" s0pair 2).
-Definition s2pair := fst (MethodBodies NatLowerUpperPairI "add" s1pair 105).
+        unfold NatSumProd_spec.
+        let f := lazymatch goal with |- ADTimpl {| MutatorMethodSpecs := ?f |} => constr:(f) end in
+            let f' := constr:(fun idx ma mb x m'a m'b => f idx (ma, mb) x (m'a, m'b)) in
+            let f'' := (eval simpl in f') in
+            let f0f1 := lazymatch f'' with
+                      | (fun idx ma mb x m'a m'b => @?f0 idx ma x m'a /\ @?f1 idx mb x m'b)
+                        => constr:((f0, f1))
+                end in
+                let AMutatorMethodSpecs := constr:(fst f0f1) in
+                let BMutatorMethodSpecs := constr:(snd f0f1) in
+                let fObs := match goal with |- ADTimpl {| ObserverMethodSpecs := ?f |} => constr:(f) end in
+                let f'Obs := constr:(fun idx ma mb x y => fObs idx (ma, mb) x y) in
+                let f''Obs := (eval simpl in f'Obs) in
+                let f0f1Obs := lazymatch f''Obs with
+                             | (fun idx ma mb x y =>
+                                  match idx with
+                                    | inl idx' => @?f0 ma x y idx'
+                                    | inr idx' => @?f1 mb x y idx'
+                                  end)
+                               => constr:((f0, f1))
+                    end in
+                    let AObserverMethodSpecs := constr:(fst f0f1Obs) in
+                    let BObserverMethodSpecs := constr:(snd f0f1Obs) in
+                    lazymatch goal with
+                  | [ |- ADTimpl
+                           {|
+                             Model := ?AModel * ?BModel;
+                             MutatorIndex := ?mutatorIndex;
+                             ObserverIndex := ?observerIndex
+                           |} ]
+                    => pose proof (@pairedImpl
+                                     (@Build_ADT AModel _ _ AMutatorMethodSpecs (fun idx' ma x y => AObserverMethodSpecs ma x y idx'))
+                                     (@Build_ADT BModel _ _ BMutatorMethodSpecs (fun idx' mb x y => BObserverMethodSpecs mb x y idx'))
+                                     mutatorIndex
+                                     observerIndex
+                                     (fun x => (x, x))
+                                     (fun x => x));
+                      unfold pairedADT in *; simpl in *
+                    end.
+                    eapply X;
+                      eauto with typeclass_instances.
+      Defined.
 
-Eval compute in snd (MethodBodies NatLowerUpperPairI "lowerBound" s2pair 0).
-Eval compute in snd (MethodBodies NatLowerUpperPairI "upperBound" s2pair 0).
+      Definition NatLowerUpper_sortOf (s : string) :=
+        if string_dec s "add"
+        then Mutator
+        else if string_dec s "lowerBound"
+             then ObserverA
+             else if string_dec s "upperBound"
+                  then ObserverB
+                  else Dummy.
 
-Definition s0prod : State NatLowerUpperProdI := (Some 10, Some 100).
-Definition s1prod := fst (MethodBodies NatLowerUpperProdI "add" s0prod 2).
-Definition s2prod := fst (MethodBodies NatLowerUpperProdI "add" s1prod 105).
+      Definition NatLowerUpperPair : ADT
+        := pairedADT (NatLower "add" "lowerBound")
+                     (NatUpper "add" "upperBound")
+                     NatLowerUpper_sortOf.
+      Definition NatLowerUpperProd : ADT
+        := prodADT (MethodSpecs (NatLower "add" "lowerBound"))
+                   (MethodSpecs (NatUpper "add" "upperBound"))
+                   NatLowerUpper_sortOf.
 
-Eval compute in snd (MethodBodies NatLowerUpperProdI "lowerBound" s2prod 0).
-Eval compute in snd (MethodBodies NatLowerUpperProdI "upperBound" s2prod 0).
+      Local Ltac pair_I_tac :=
+        repeat match goal with
+                 | _ => intro
+                 | _ => progress simpl in *
+                 | [ |- context[if ?E then _ else _ ] ] => destruct E; subst
+               end;
+        simpl; unfold mutator, observer; simpl; instantiate; firstorder (subst; eauto).
+
+      Definition NatLowerUpperPairI : ADTimpl NatLowerUpperPair.
+        refine (pairedImpl NatLowerUpper_sortOf
+                           (NatLowerI "add" "lowerBound" I)
+                           (NatUpperI "add" "upperBound" I)
+                           _);
+        unfold NatLowerUpper_sortOf.
+        abstract pair_I_tac.
+      Defined.
+
+      Definition NatLowerUpperProdI : ADTimpl NatLowerUpperProd.
+        refine (prodImpl NatLowerUpper_sortOf
+                         (NatLowerI "add" "lowerBound" I)
+                         (NatUpperI "add" "upperBound" I)
+                         _
+                         _);
+        unfold NatLowerUpper_sortOf;
+        abstract pair_I_tac.
+      Defined.
 
 
 
-Definition NatSumProd_sortOf (s : string) :=
-  if string_dec s "add"
-  then Mutator
-  else if string_dec s "sum"
-       then ObserverA
-       else if string_dec s "prod"
-            then ObserverB
-            else Dummy.
+      Definition s0pair : State NatLowerUpperPairI := (Some 10, Some 100).
+      Definition s1pair := fst (MethodBodies NatLowerUpperPairI "add" s0pair 2).
+      Definition s2pair := fst (MethodBodies NatLowerUpperPairI "add" s1pair 105).
 
-Definition NatSumProdPair : ADT
-  := pairedADT (NatSum "add" "sum")
-               (NatProd "add" "prod")
-               NatSumProd_sortOf.
-Definition NatSumProdProd : ADT
-  := prodADT (MethodSpecs (NatSum "add" "sum"))
-             (MethodSpecs (NatProd "add" "prod"))
-             NatSumProd_sortOf.
+      Eval compute in snd (MethodBodies NatLowerUpperPairI "lowerBound" s2pair 0).
+      Eval compute in snd (MethodBodies NatLowerUpperPairI "upperBound" s2pair 0).
 
-Definition NatSumProdPairI : ADTimpl NatSumProdPair.
-  refine (pairedImpl NatSumProd_sortOf
-                     (NatSumI "add" "sum" I)
-                     (NatProdI "add" "prod" I)
-                     _);
-  unfold NatSumProd_sortOf;
-  abstract pair_I_tac.
-Defined.
+      Definition s0prod : State NatLowerUpperProdI := (Some 10, Some 100).
+      Definition s1prod := fst (MethodBodies NatLowerUpperProdI "add" s0prod 2).
+      Definition s2prod := fst (MethodBodies NatLowerUpperProdI "add" s1prod 105).
 
-Definition NatSumProdProdI : ADTimpl NatSumProdProd.
-  refine (prodImpl NatSumProd_sortOf
-                   (NatSumI "add" "sum" I)
-                   (NatProdI "add" "prod" I)
-                   _
-                   _);
-  unfold NatSumProd_sortOf;
-  abstract pair_I_tac.
-Defined.
+      Eval compute in snd (MethodBodies NatLowerUpperProdI "lowerBound" s2prod 0).
+      Eval compute in snd (MethodBodies NatLowerUpperProdI "upperBound" s2prod 0).
 
-Definition s0'pair : State NatSumProdPairI := (Some 10, Some 100).
-Definition s1'pair := fst (MethodBodies NatSumProdPairI "add" s0'pair 2).
-Definition s2'pair := fst (MethodBodies NatSumProdPairI "add" s1'pair 105).
 
-Eval compute in snd (MethodBodies NatSumProdPairI "sum" s2'pair 0).
-Eval compute in snd (MethodBodies NatSumProdPairI "prod" s2'pair 0).
 
-Definition s0'prod : State NatSumProdProdI := (Some 10, Some 100).
-Definition s1'prod := fst (MethodBodies NatSumProdProdI "add" s0'prod 2).
-Definition s2'prod := fst (MethodBodies NatSumProdProdI "add" s1'prod 105).
+      Definition NatSumProd_sortOf (s : string) :=
+        if string_dec s "add"
+        then Mutator
+        else if string_dec s "sum"
+             then ObserverA
+             else if string_dec s "prod"
+                  then ObserverB
+                  else Dummy.
 
-Eval compute in snd (MethodBodies NatSumProdProdI "sum" s2'prod 0).
-Eval compute in snd (MethodBodies NatSumProdProdI "prod" s2'prod 0).
-     *)
+      Definition NatSumProdPair : ADT
+        := pairedADT (NatSum "add" "sum")
+                     (NatProd "add" "prod")
+                     NatSumProd_sortOf.
+      Definition NatSumProdProd : ADT
+        := prodADT (MethodSpecs (NatSum "add" "sum"))
+                   (MethodSpecs (NatProd "add" "prod"))
+                   NatSumProd_sortOf.
+
+      Definition NatSumProdPairI : ADTimpl NatSumProdPair.
+        refine (pairedImpl NatSumProd_sortOf
+                           (NatSumI "add" "sum" I)
+                           (NatProdI "add" "prod" I)
+                           _);
+        unfold NatSumProd_sortOf;
+        abstract pair_I_tac.
+      Defined.
+
+      Definition NatSumProdProdI : ADTimpl NatSumProdProd.
+        refine (prodImpl NatSumProd_sortOf
+                         (NatSumI "add" "sum" I)
+                         (NatProdI "add" "prod" I)
+                         _
+                         _);
+        unfold NatSumProd_sortOf;
+        abstract pair_I_tac.
+      Defined.
+
+      Definition s0'pair : State NatSumProdPairI := (Some 10, Some 100).
+      Definition s1'pair := fst (MethodBodies NatSumProdPairI "add" s0'pair 2).
+      Definition s2'pair := fst (MethodBodies NatSumProdPairI "add" s1'pair 105).
+
+      Eval compute in snd (MethodBodies NatSumProdPairI "sum" s2'pair 0).
+      Eval compute in snd (MethodBodies NatSumProdPairI "prod" s2'pair 0).
+
+      Definition s0'prod : State NatSumProdProdI := (Some 10, Some 100).
+      Definition s1'prod := fst (MethodBodies NatSumProdProdI "add" s0'prod 2).
+      Definition s2'prod := fst (MethodBodies NatSumProdProdI "add" s1'prod 105).
+
+      Eval compute in snd (MethodBodies NatSumProdProdI "sum" s2'prod 0).
+      Eval compute in snd (MethodBodies NatSumProdProdI "prod" s2'prod 0).
+      *)
+*)
